SeparationLogic/examples/QCP_demos_LLM/kosaraju_rel_proof_auto.v
@@ -23,16 +23,8 @@ Export MonadNotation.
 Local Open Scope monad.
 From AUXLib Require Import int_auto Axioms Feq Idents ListLib VMap relations.
 From FP Require Import PartialOrder_Setoid BourbakiWitt.
-Require Import SimpleC.EE.QCP_demos_LLM.sll_lib.
-Require Import SimpleC.EE.QCP_demos_LLM.SllPtrArrayLib.
 Require Import SimpleC.EE.QCP_demos_LLM.kosaraju_rel_lib.
 Local Open Scope sac.
-
-Lemma proof_of_kosaraju_num_vertices_return_wit_1 : kosaraju_num_vertices_return_wit_1.
-Proof. Admitted. 
-
-Lemma proof_of_kosaraju_get_visited1_partial_solve_wit_1 : kosaraju_get_visited1_partial_solve_wit_1.
-Proof. Admitted. 
 
 Lemma proof_of_dfs1_safety_wit_1 : dfs1_safety_wit_1.
 Proof. Admitted. 
@@ -49,7 +41,22 @@ Proof. Admitted.
 Lemma proof_of_dfs1_safety_wit_5 : dfs1_safety_wit_5.
 Proof. Admitted. 
 
+Lemma proof_of_dfs1_safety_wit_6 : dfs1_safety_wit_6.
+Proof. Admitted. 
+
 Lemma proof_of_dfs1_safety_wit_7 : dfs1_safety_wit_7.
+Proof. Admitted. 
+
+Lemma proof_of_dfs1_safety_wit_8 : dfs1_safety_wit_8.
+Proof. Admitted. 
+
+Lemma proof_of_dfs1_safety_wit_9 : dfs1_safety_wit_9.
+Proof. Admitted. 
+
+Lemma proof_of_dfs1_safety_wit_10 : dfs1_safety_wit_10.
+Proof. Admitted. 
+
+Lemma proof_of_dfs1_safety_wit_12 : dfs1_safety_wit_12.
 Proof. Admitted. 
 
 Lemma proof_of_dfs1_partial_solve_wit_1 : dfs1_partial_solve_wit_1.
@@ -59,9 +66,6 @@ Lemma proof_of_dfs1_partial_solve_wit_2 : dfs1_partial_solve_wit_2.
 Proof. Admitted. 
 
 Lemma proof_of_dfs1_partial_solve_wit_3 : dfs1_partial_solve_wit_3.
-Proof. Admitted. 
-
-Lemma proof_of_dfs1_partial_solve_wit_4_pure : dfs1_partial_solve_wit_4_pure.
 Proof. Admitted. 
 
 Lemma proof_of_dfs1_partial_solve_wit_4 : dfs1_partial_solve_wit_4.
@@ -76,6 +80,12 @@ Proof. Admitted.
 Lemma proof_of_dfs1_partial_solve_wit_7 : dfs1_partial_solve_wit_7.
 Proof. Admitted. 
 
+Lemma proof_of_dfs1_partial_solve_wit_8 : dfs1_partial_solve_wit_8.
+Proof. Admitted. 
+
+Lemma proof_of_dfs1_partial_solve_wit_9 : dfs1_partial_solve_wit_9.
+Proof. Admitted. 
+
 Lemma proof_of_dfs2_safety_wit_1 : dfs2_safety_wit_1.
 Proof. Admitted. 
 
@@ -83,6 +93,21 @@ Lemma proof_of_dfs2_safety_wit_2 : dfs2_safety_wit_2.
 Proof. Admitted. 
 
 Lemma proof_of_dfs2_safety_wit_3 : dfs2_safety_wit_3.
+Proof. Admitted. 
+
+Lemma proof_of_dfs2_safety_wit_4 : dfs2_safety_wit_4.
+Proof. Admitted. 
+
+Lemma proof_of_dfs2_safety_wit_5 : dfs2_safety_wit_5.
+Proof. Admitted. 
+
+Lemma proof_of_dfs2_safety_wit_6 : dfs2_safety_wit_6.
+Proof. Admitted. 
+
+Lemma proof_of_dfs2_safety_wit_7 : dfs2_safety_wit_7.
+Proof. Admitted. 
+
+Lemma proof_of_dfs2_safety_wit_8 : dfs2_safety_wit_8.
 Proof. Admitted. 
 
 Lemma proof_of_dfs2_partial_solve_wit_1 : dfs2_partial_solve_wit_1.
@@ -100,81 +125,12 @@ Proof. Admitted.
 Lemma proof_of_dfs2_partial_solve_wit_5 : dfs2_partial_solve_wit_5.
 Proof. Admitted. 
 
-Lemma proof_of_dfs2_partial_solve_wit_6_pure : dfs2_partial_solve_wit_6_pure.
-Proof. Admitted. 
-
 Lemma proof_of_dfs2_partial_solve_wit_6 : dfs2_partial_solve_wit_6.
 Proof. Admitted. 
 
-Lemma proof_of_kosaraju_finish_safety_wit_1 : kosaraju_finish_safety_wit_1.
+Lemma proof_of_dfs2_partial_solve_wit_7 : dfs2_partial_solve_wit_7.
 Proof. Admitted. 
 
-Lemma proof_of_kosaraju_finish_safety_wit_2 : kosaraju_finish_safety_wit_2.
-Proof. Admitted. 
-
-Lemma proof_of_kosaraju_finish_safety_wit_3 : kosaraju_finish_safety_wit_3.
-Proof. Admitted. 
-
-Lemma proof_of_kosaraju_finish_safety_wit_4 : kosaraju_finish_safety_wit_4.
-Proof. Admitted. 
-
-Lemma proof_of_kosaraju_finish_partial_solve_wit_1 : kosaraju_finish_partial_solve_wit_1.
-Proof. Admitted. 
-
-Lemma proof_of_kosaraju_finish_partial_solve_wit_2_pure : kosaraju_finish_partial_solve_wit_2_pure.
-Proof. Admitted. 
-
-Lemma proof_of_kosaraju_finish_partial_solve_wit_2 : kosaraju_finish_partial_solve_wit_2.
-Proof. Admitted. 
-
-Lemma proof_of_kosaraju_scc_safety_wit_1 : kosaraju_scc_safety_wit_1.
-Proof. Admitted. 
-
-Lemma proof_of_kosaraju_scc_safety_wit_2 : kosaraju_scc_safety_wit_2.
-Proof. Admitted. 
-
-Lemma proof_of_kosaraju_scc_safety_wit_3 : kosaraju_scc_safety_wit_3.
-Proof. Admitted. 
-
-Lemma proof_of_kosaraju_scc_safety_wit_4 : kosaraju_scc_safety_wit_4.
-Proof. Admitted. 
-
-Lemma proof_of_kosaraju_scc_safety_wit_6 : kosaraju_scc_safety_wit_6.
-Proof. Admitted. 
-
-Lemma proof_of_kosaraju_scc_safety_wit_7 : kosaraju_scc_safety_wit_7.
-Proof. Admitted. 
-
-Lemma proof_of_kosaraju_scc_safety_wit_8 : kosaraju_scc_safety_wit_8.
-Proof. Admitted. 
-
-Lemma proof_of_kosaraju_scc_safety_wit_9 : kosaraju_scc_safety_wit_9.
-Proof. Admitted. 
-
-Lemma proof_of_kosaraju_scc_partial_solve_wit_1 : kosaraju_scc_partial_solve_wit_1.
-Proof. Admitted. 
-
-Lemma proof_of_kosaraju_scc_partial_solve_wit_2 : kosaraju_scc_partial_solve_wit_2.
-Proof. Admitted. 
-
-Lemma proof_of_kosaraju_scc_partial_solve_wit_3 : kosaraju_scc_partial_solve_wit_3.
-Proof. Admitted. 
-
-Lemma proof_of_kosaraju_scc_partial_solve_wit_4 : kosaraju_scc_partial_solve_wit_4.
-Proof. Admitted. 
-
-Lemma proof_of_kosaraju_scc_partial_solve_wit_5 : kosaraju_scc_partial_solve_wit_5.
-Proof. Admitted. 
-
-Lemma proof_of_kosaraju_scc_partial_solve_wit_6 : kosaraju_scc_partial_solve_wit_6.
-Proof. Admitted. 
-
-Lemma proof_of_kosaraju_scc_partial_solve_wit_7 : kosaraju_scc_partial_solve_wit_7.
-Proof. Admitted. 
-
-Lemma proof_of_kosaraju_run_partial_solve_wit_1 : kosaraju_run_partial_solve_wit_1.
-Proof. Admitted. 
-
-Lemma proof_of_kosaraju_run_partial_solve_wit_2 : kosaraju_run_partial_solve_wit_2.
+Lemma proof_of_dfs2_partial_solve_wit_8 : dfs2_partial_solve_wit_8.
 Proof. Admitted. 
 
